cleanup

extra/SepROExtra.v
@@ -13,7 +13,7 @@ Lemma to_ro_duplicatable : forall h,
   duplicatable (= to_ro h).
 Proof using.
   intros h. unfolds. intros h' E. subst.
-  lets D: heap_compat_refl_to_ro h. do 2 esplit. splits*. 
+  lets D: heap_compat_refl_to_ro h. do 2 esplit. splits*.
   rewrite* heap_union_eq_of_compat. rewrite* union_same.
 Qed.
 
@@ -24,16 +24,16 @@ Qed.
 
 Lemma decomposition : forall H,
   H ==> (\exists H1 H2, \[Normal H1 /\ (haffine H -> haffine H1)]
-                     \* \[ReadOnly H2] \* (H1 \* H2)). 
+                     \* \[ReadOnly H2] \* (H1 \* H2)).
 Proof using.
   intros H h K. rewrite (heap_eq_union_rw_ro h).
   exists (= h^rw) (= h^ro). do 2 rewrite hstar_hpure. splits.
-  { splits. 
+  { splits.
     { intros ? ->. rew_heap*. }
     { intros F. Transparent haffine. unfolds haffine. intros ? ->.
-      specializes F K. rewrite (heap_eq_union_rw_ro h) in F. 
+      specializes F K. rewrite (heap_eq_union_rw_ro h) in F.
       forwards*: heap_affine_union_inv F. } }
-  { intros ? ->. rew_heap*. } 
+  { intros ? ->. rew_heap*. }
   { do 2 esplit. splits*. }
 Qed.
 
@@ -45,7 +45,7 @@ Proof using.
   introv M.
   forwards K: decomposition H'.
   lets WH: himpl_frame_r H K.
-  applys* triple_conseq WH. 
+  applys* triple_conseq WH.
   rewrite hstar_comm. (* manual xpull *)
   rewrite hstar_hexists. applys triple_hexists. intros H1.
   rewrite hstar_hexists. applys triple_hexists. intros H2.
@@ -106,7 +106,7 @@ Lemma agree_filter_mode : forall h1 h2 m1 m2,
   agree h1 h2 ->
   agree (filter_mode m1 h1) (filter_mode m2 h2).
 Proof using.
-  introv D. intros l v1 v2 E1 E2. 
+  introv D. intros l v1 v2 E1 E2.
   unfold filter_mode in *. intros x M1 M2.
   rewrite (@indom_filter_eq _ _ val_mode_inhab) in M1,M2.
   false*.
@@ -155,7 +155,7 @@ Qed.
 
 Lemma RO_RO : forall H,
   RO (RO H) = RO H.
-Proof using. 
+Proof using.
   intros. unfold RO. applys himpl_antisym.
   { xpull ;=> h' R.
     lets (h''&R'): hexists_inv (rm R).
@@ -163,7 +163,162 @@ Proof using.
     rewrite to_ro_idempotent. xsimpl*. }
   { xpull ;=> h' R. xsimpl (to_ro h').
     { applys hexists_intro h'. rewrite* hstar_hpure_l. }
-    { rewrite* to_ro_idempotent. } } 
+    { rewrite* to_ro_idempotent. } }
 Qed.
 *)
 
+
+
+
+(* TODO:
+
+Module FMaps.
+Section Map.
+Transparent Fmap.map.
+(* TODO: this function only maps values, we'd need another function to map keys as well *)
+
+Program Definition map_ A B1 B2 `{Inhab B1} `{Inhab B2} (f:A->B1->B2) (M:fmap A B1) : fmap A B2 :=
+  Fmap.make (fun (x:A) => match Fmap.read M x with
+    | None => None
+    | Some y => Some (f x y)
+    end) _.
+(*
+Transparent update (*update_inst*) bag_update_as_union_single single_bind single_bind_inst LibMap.union_inst LibContainer.union.
+*)
+Lemma map_update : forall A `{Inhab B1} `{Inhab B2} (f:A->B1->B2) (M:Fmap.map A B1) x y,
+  map_ f (Fmap.update M x y) = Fmap.update (map_ f M) x (f x y).
+Proof using.
+  intros. extens. intros a. unfold map_. simpl. unfold bag_update_as_union_single.
+  unfold single_bind. simpl. unfold single_bind_impl. unfold LibContainer.union. simpl.
+  unfold LibMap.union_impl.
+  case_if; subst. autos*. destruct* (M a). (* TODO: cleanup *)
+Qed.
+
+Transparent dom dom_inst.
+
+Lemma dom_map : forall A `{Inhab B1} `{Inhab B2} (f:A->B1->B2) (M:map A B1),
+  dom (map_ f M) = dom M.
+Proof using.
+  intros. unfold map_. simpl. unfold dom_impl.
+  fequal. extens. intros x. destruct (M x); auto_false.
+Qed.
+
+Transparent read LibMap.read_inst.
+
+Lemma read_map : forall A `{Inhab B1} `{Inhab B2} (f:A->B1->B2) (M:map A B1) (x:A),
+  x \indom M ->
+  (map_ f M)[x] = f x (M[x]).
+Proof using.
+  introv Hx. unfold map_. simpl. unfold read, LibMap.read_inst. unfold LibMap.read_impl.
+  unfold dom, LibMap.dom_inst, dom_impl in Hx. rewrite in_set_st_eq in Hx.
+  destruct (M x); auto_false.
+Qed.
+
+Axiom extens : forall A `{Inhab B} (M1 M2:map A B),
+  dom M1 = dom M2 ->
+  (forall (x:A), x \indom M1 -> M1[x] = M2[x]) ->
+  M1 = M2.
+
+End Map.
+
+Section Filter.
+Transparent map.
+
+Definition filter A `{Inhab B} (f:A->B->Prop) (M:map A B) : map A B :=
+  fun (x:A) => match M x with
+    | None => None
+    | Some y => If f x y then Some y else None
+    end.
+
+Transparent update bag_update_as_union_single single_bind single_bind_inst LibMap.union_inst LibContainer.union.
+
+Transparent dom dom_inst.
+
+Lemma dom_filter : forall A `{Inhab B} (f:A->B->Prop) (M:map A B),
+  dom (filter f M) \c dom M.
+Proof using.
+Admitted.
+
+Transparent read LibMap.read_inst.
+
+Lemma read_filter : forall A `{Inhab B} (f:A->B->Prop) (M:map A B) x,
+  x \indom M ->
+  f x (M[x]) ->
+  (filter f M)[x] = M[x].
+Proof using.
+Admitted.
+
+End Filter.
+
+End FMaps.
+*)
+
+
+
+(* Hint Resolve Fmap.agree_sym. *)
+
+
+(* TODO: check what's actually needed *)
+Lemma heap_eq_forward : forall h1 h2,
+  h1 = h2 ->
+  h1^rw = h2^rw /\ h1^ro = h2^ro.
+Proof using. intros. subst*. Qed.
+
+
+
+(* ---------------------------------------------------------------------- *)
+(* ** Equalities on heaps *)
+
+Lemma heap_eq : forall h1 h2,
+  h1^rw = h2^rw ->
+  h1^ro = h2^ro ->
+  h1 = h2.
+Proof using.
+  introv M1 M2. forwards (E1&_): heap_eq_disjoint_union_rw_ro h1.
+  forwards (E2&_): heap_eq_disjoint_union_rw_ro h2. congruence.
+Qed.
+
+
+(* ---------------------------------------------------------------------- *)
+(* ** Properties of [heap_empty] *)
+
+(* not needed
+Lemma heap_empty_state : heap_state heap_empty = Fmap.empty.
+Proof using.
+  unfold heap_empty. unfold heap_state. rewrite* map_empty.
+Qed.
+
+Hint Rewrite heap_empty_state : rew_heap.
+*)
+
+
+(* not needed? *)
+Lemma heap_union_state : forall h1 h2,
+  heap_compat h1 h2 ->
+  heap_state (h1 \u h2) = heap_state h1 \+ heap_state h2.
+Proof using. introv D. rew_fmap*. Qed.
+
+
+
+(* ---------------------------------------------------------------------- *)
+(* ** Properties  *)
+
+Lemma heap_state_components : forall h,
+  heap_state h = heap_state (h^rw) \+ heap_state (h^ro).
+Proof using.
+  intros. lets (E&D): heap_eq_disjoint_union_rw_ro h.
+  rewrite E at 1. rew_fmap*. applys* heap_compat_of_disjoint.
+Qed.
+
+
+(*
+Lemma hgc_intro : forall h,
+  \GC h.
+Proof using. intros. applys hgc_of_heap_affine. hnfs*. Qed.
+*)
+
+
+(* equivalent to:
+Definition RO' (H:hprop) : hprop :=
+  \exists h', \[H h'] \* (= to_ro h').
+ *)
